src/axiomatic/PFtoA3.v
@@ -1,0 +1,245 @@
+Require Import Relations.
+Require Import Permutation.
+Require Import NArith.
+Require Import PArith.
+Require Import ZArith.
+Require Import Lia.
+Require Import FMapPositive.
+Require Import FSetPositive.
+Require Import EquivDec.
+Require Import sflib.
+Require Import paco.
+Require Import HahnRelationsBasic.
+Require Import HahnSets.
+
+Require Import PromisingArch.lib.Basic.
+Require Import PromisingArch.lib.HahnRelationsMore.
+Require Import PromisingArch.lib.Order.
+Require Import PromisingArch.lib.Time.
+Require Import PromisingArch.lib.Lang.
+Require Import PromisingArch.promising.Promising.
+Require Import PromisingArch.promising.StateExecFacts.
+Require Import PromisingArch.axiomatic.Axiomatic.
+Require Import PromisingArch.axiomatic.CommonAxiomatic.
+Require Import PromisingArch.axiomatic.PFtoA1.
+Require Import PromisingArch.axiomatic.PFtoA2.
+
+Set Implicit Arguments.
+
+
+Definition ob' (ex: Execution.t): relation eidT :=
+  ex.(Execution.rfe) ∪ ex.(Execution.dob) ∪ ex.(Execution.aob) ∪ ex.(Execution.bob).
+
+Ltac des_union :=
+  repeat
+    (try match goal with
+         | [H: Execution.internal _ _ _ |- _] => inv H
+         | [H: Execution.ob _ _ _ |- _] => inv H
+         | [H: Execution.obs _ _ _ |- _] => inv H
+         | [H: (_ ∪ _) _ _ |- _] => inv H
+         end).
+
+Lemma ob_ob'
+      ex eid1 eid2:
+  ex.(Execution.ob) eid1 eid2 <->
+  (ex.(Execution.fr) ∪ ex.(Execution.co) ∪ ex.(ob')) eid1 eid2.
+Proof.
+  split; i.
+  - des_union.
+    + right. left. left. left. auto.
+    + left. left. auto.
+    + left. right. auto.
+    + right. left. left. right. auto.
+    + right. left. right. auto.
+    + right. right. auto.
+  - unfold ob' in *. des_union.
+    + left. left. left. left. right. auto.
+    + left. left. left. right. auto.
+    + left. left. left. left. left. auto.
+    + left. left. right. auto.
+    + left. right. auto.
+    + right. auto.
+Qed.
+
+Lemma nth_error_last A (l: list A) a n
+      (N: Nat.eqb n (List.length l) = true):
+  List.nth_error (l ++ [a]) n = Some a.
+Proof.
+  apply Nat.eqb_eq in N. subst.
+  rewrite List.nth_error_app2, Nat.sub_diag; ss. 
+Qed.
+
+Lemma nth_error_not_last A (l: list A) a b n
+      (NTH: List.nth_error (l ++ [a]) n = Some b)
+      (N: Nat.eqb n (List.length l) = false):
+  n < List.length l.
+Proof.
+  apply nth_error_snoc_inv in NTH. des; ss. subst.
+  apply Nat.eqb_neq in N. lia.
+Qed.
+
+Definition sim_view (vext: eidT -> Time.t) (view: Time.t) (eids: eidT -> Prop): Prop :=
+  forall eid (EID: eids eid), le (vext eid) view.
+
+Inductive sim_view_rev (vext: eidT -> Time.t) (view: Time.t) (eids: eidT -> Prop): Prop :=
+| sim_view_rev_bot
+    (VIEW: view = bot)
+| sim_view_rev_event
+    eid
+    (EID: eids eid)
+    (VIEW: le view (vext eid))
+.
+Hint Constructors sim_view_rev.
+
+Definition sim_view_eq (vext: eidT -> Time.t) (view: Time.t) (eids: eidT -> Prop): Prop :=
+  sim_view vext view eids /\ sim_view_rev vext view eids.
+
+Inductive sim_val (tid:Id.t) (vext:eidT -> Time.t) (vala:ValA.t (A:=View.t (A:=unit))) (avala:ValA.t (A:=nat -> Prop)): Prop :=
+| sim_val_intro
+    (VAL: vala.(ValA.val) = avala.(ValA.val))
+    (VIEW: sim_view vext vala.(ValA.annot).(View.ts) (fun eid => eid.(fst) = tid /\ avala.(ValA.annot) eid.(snd)))
+.
+Hint Constructors sim_val.
+
+Inductive sim_rmap (tid:Id.t) (vext:eidT -> Time.t) (rmap:RMap.t (A:=View.t (A:=unit))) (armap:RMap.t (A:=nat -> Prop)): Prop :=
+| sim_rmap_intro
+    (RMAP: IdMap.Forall2 (fun reg => sim_val tid vext) rmap armap)
+.
+Hint Constructors sim_rmap.
+
+Inductive sim_state (tid:Id.t) (vext:eidT -> Time.t) (state:State.t (A:=View.t (A:=unit))) (astate:State.t (A:=nat -> Prop)): Prop :=
+| sim_state_intro
+    (STMTS: state.(State.stmts) = astate.(State.stmts))
+    (RMAP: sim_rmap tid vext state.(State.rmap) astate.(State.rmap))
+.
+Hint Constructors sim_state.
+
+Lemma sim_rmap_add
+      tid vext rmap armap reg vala avala
+      (SIM: sim_rmap tid vext rmap armap)
+      (VAL: sim_val tid vext vala avala):
+  sim_rmap tid vext (RMap.add reg vala rmap) (RMap.add reg avala armap).
+Proof.
+  econs. ii. unfold RMap.add. rewrite ? IdMap.add_spec.
+  inv SIM. condtac; eauto.
+Qed.
+
+Lemma sim_rmap_expr
+      tid vext rmap armap e
+      (SIM: sim_rmap tid vext rmap armap):
+  sim_val tid vext (sem_expr rmap e) (sem_expr armap e).
+Proof.
+  inv SIM. induction e; s.
+  - (* const *)
+    econs; ss. ii. inv EID. inv H0.
+  - (* reg *)
+    specialize (RMAP reg). unfold RMap.find. inv RMAP; ss.
+    econs; ss. ii. inv EID. inv H2.
+  - (* op1 *)
+    inv IHe. econs; ss. congr.
+  - (* op2 *)
+    inv IHe1. inv IHe2. econs; ss.
+    + congr.
+    + ii. des. inv EID0.
+      * etrans; [|eapply join_l]; eauto.
+      * etrans; [|eapply join_r]; eauto.
+Qed.
+
+Inductive sim_local (tid:Id.t) (ex: Execution.t) (vext: eidT -> Time.t) (local:Local.t (A:=unit)) (alocal:ALocal.t): Prop := mk_sim_local {
+  COH: forall loc,
+        sim_view
+          vext
+          (local.(Local.coh) loc)
+          (inverse (sim_local_coh ex loc) (eq (tid, List.length (alocal.(ALocal.labels)))));
+  VRP: sim_view
+         vext
+         local.(Local.vrp).(View.ts)
+         (inverse (sim_local_vrp ex) (eq (tid, List.length (alocal.(ALocal.labels)))));
+  VWP: sim_view
+         vext
+         local.(Local.vwp).(View.ts)
+         (inverse (sim_local_vwp ex) (eq (tid, List.length (alocal.(ALocal.labels)))));
+  VRM: sim_view
+         vext
+         local.(Local.vrm).(View.ts)
+         (inverse (sim_local_vrm ex) (eq (tid, List.length (alocal.(ALocal.labels)))));
+  VWM: sim_view
+         vext
+         local.(Local.vwm).(View.ts)
+         (inverse (sim_local_vwm ex) (eq (tid, List.length (alocal.(ALocal.labels)))));
+  VCAP: sim_view
+          vext
+          local.(Local.vcap).(View.ts)
+          (inverse (sim_local_vcap ex) (eq (tid, List.length (alocal.(ALocal.labels)))));
+  VREL: sim_view
+          vext
+          local.(Local.vrel).(View.ts)
+          (inverse (sim_local_vrel ex) (eq (tid, List.length (alocal.(ALocal.labels)))));
+  FWDBANK: forall loc,
+      (exists eid,
+          <<TS_NONZERO: (local.(Local.fwdbank) loc).(FwdItem.ts) > 0>> /\
+          <<WRITE: sim_local_fwd ex loc eid (tid, List.length (alocal.(ALocal.labels)))>> /\
+          <<TS: vext eid = (local.(Local.fwdbank) loc).(FwdItem.ts)>> /\
+          <<VIEW: sim_view
+                    vext
+                    (local.(Local.fwdbank) loc).(FwdItem.view).(View.ts)
+                    (inverse (ex.(Execution.addr) ∪ ex.(Execution.data)) (eq eid))>> /\
+          <<EX: (local.(Local.fwdbank) loc).(FwdItem.ex) <-> ex.(Execution.label_is) (Label.is_ex) eid>>) \/
+      ((local.(Local.fwdbank) loc) = FwdItem.init /\
+       forall eid, ~ (inverse (sim_local_fwd_none ex loc) (eq (tid, List.length (alocal.(ALocal.labels)))) eid));
+  EXBANK: opt_rel
+            (fun aeb eb =>
+               ex.(Execution.label_is) (Label.is_reading eb.(Exbank.loc)) (tid, aeb) /\
+               sim_view_eq
+                 vext
+                 eb.(Exbank.ts)
+                 (inverse ex.(Execution.rf) (eq (tid, aeb))) /\
+               sim_view
+                 vext
+                 eb.(Exbank.view).(View.ts)
+                 (eq (tid, aeb)))
+            alocal.(ALocal.exbank) local.(Local.exbank);
+  PROMISES: forall view (VIEW: Promises.lookup view local.(Local.promises)),
+      exists n,
+        <<N: (length alocal.(ALocal.labels)) <= n>> /\
+        <<WRITE: ex.(Execution.label_is) Label.is_write (tid, n)>> /\
+        <<VIEW: vext (tid, n) = view>>;
+}.
+Hint Constructors sim_local.
+
+Definition sim_ob_write
+           (tid:Id.t) (ex:Execution.t) (vext: eidT -> Time.t)
+           (eu:ExecUnit.t (A:=unit)) (aeu:AExecUnit.t): Prop :=
+  forall eid1 eid2
+    (LABEL: eid2 < List.length aeu.(AExecUnit.local).(ALocal.labels))
+    (OB: ex.(ob') eid1 (tid, eid2))
+    (EID2: ex.(Execution.label_is) Label.is_write (tid, eid2)),
+    Time.lt (vext eid1) (vext (tid, eid2)).
+
+Definition sim_ob_read
+           (tid:Id.t) (ex:Execution.t) (vext: eidT -> Time.t)
+           (eu:ExecUnit.t (A:=unit)) (aeu:AExecUnit.t): Prop :=
+  forall eid1 eid2
+    (LABEL: eid2 < List.length aeu.(AExecUnit.local).(ALocal.labels))
+    (AOB: ex.(ob') eid1 (tid, eid2))
+    (EID2: ex.(Execution.label_is) Label.is_read (tid, eid2)),
+    Time.le (vext eid1) (vext (tid, eid2)).
+
+Definition sim_fr
+           (tid:Id.t) (ex:Execution.t) (vext: eidT -> Time.t)
+           (eu:ExecUnit.t (A:=unit)) (aeu:AExecUnit.t): Prop :=
+  forall eid1 eid2
+    (LABEL: eid1 < List.length aeu.(AExecUnit.local).(ALocal.labels))
+    (FR: ex.(Execution.fr) (tid, eid1) eid2),
+    Time.lt (vext (tid, eid1)) (vext eid2).
+
+Inductive sim_th'
+          (tid:Id.t) (ex:Execution.t) (vext: eidT -> Time.t)
+          (eu:ExecUnit.t (A:=unit)) (aeu:AExecUnit.t): Prop := {
+  ST: sim_state tid vext eu.(ExecUnit.state) aeu.(AExecUnit.state);
+  LC: sim_local tid ex vext eu.(ExecUnit.local) aeu.(AExecUnit.local);
+  OBW: sim_ob_write tid ex vext eu aeu;
+  OBR: sim_ob_read tid ex vext eu aeu;
+  FR: sim_fr tid ex vext eu aeu;
+}.
+Hint Constructors sim_th'.
