src/axiomatic/PFtoA4FR.v
@@ -1,0 +1,167 @@
+Require Import Relations.
+Require Import Permutation.
+Require Import NArith.
+Require Import PArith.
+Require Import ZArith.
+Require Import Lia.
+Require Import FMapPositive.
+Require Import FSetPositive.
+Require Import EquivDec.
+Require Import sflib.
+Require Import paco.
+Require Import HahnRelationsBasic.
+Require Import HahnSets.
+
+Require Import PromisingArch.lib.Basic.
+Require Import PromisingArch.lib.HahnRelationsMore.
+Require Import PromisingArch.lib.Order.
+Require Import PromisingArch.lib.Time.
+Require Import PromisingArch.lib.Lang.
+Require Import PromisingArch.promising.Promising.
+Require Import PromisingArch.promising.StateExecFacts.
+Require Import PromisingArch.axiomatic.Axiomatic.
+Require Import PromisingArch.axiomatic.CommonAxiomatic.
+Require Import PromisingArch.axiomatic.PFtoA1.
+Require Import PromisingArch.axiomatic.PFtoA2.
+Require Import PromisingArch.axiomatic.PFtoA3.
+
+Set Implicit Arguments.
+
+
+Lemma sim_traces_sim_th'_fr
+      p trs atrs ws rs covs vexts
+      m ex
+      (STEP: Machine.pf_exec p m)
+      (SIM: sim_traces p m.(Machine.mem) trs atrs ws rs covs vexts)
+      (PRE: Valid.pre_ex p ex)
+      (CO: ex.(Execution.co) = co_gen ws)
+      (RF: ex.(Execution.rf) = rf_gen ws rs)
+      (CO1: Valid.co1 ex)
+      (CO2: Valid.co2 ex)
+      (RF1: Valid.rf1 ex)
+      (RF2: Valid.rf2 ex)
+      (RF_WF: Valid.rf_wf ex)
+      (TR: IdMap.Forall2
+             (fun _ tr sl => exists l, tr = (ExecUnit.mk sl.(fst) sl.(snd) m.(Machine.mem)) :: l)
+             trs m.(Machine.tpool))
+      (ATR: IdMap.Forall2
+              (fun _ atr aeu => exists l, atr = aeu :: l)
+              atrs (Valid.aeus PRE)):
+  forall tid tr atr covl vextl
+    n eu1 eu2 tr' aeu1 aeu2 atr' cov1 cov2 covl' vext1 vext2 vextl'
+    (FIND_TR: IdMap.find tid trs = Some tr)
+    (FIND_ATR: IdMap.find tid atrs = Some atr)
+    (FIND_COVL: IdMap.find tid covs = Some covl)
+    (FIND_VEXTL: IdMap.find tid vexts = Some vextl)
+    (EU: lastn (S n) tr = eu2 :: eu1 :: tr')
+    (AEU: lastn (S n) atr = aeu2 :: aeu1 :: atr')
+    (COV: lastn (S n) covl = cov2 :: cov1 :: covl')
+    (VEXT: lastn (S n) vextl = vext2 :: vext1 :: vextl')
+    (SIM_TH': sim_th' tid ex (v_gen vexts) eu1 aeu1),
+    sim_fr tid ex (v_gen vexts) eu2 aeu2.
+Proof.
+  i. rename SIM_TH' into L.
+  generalize (SIM tid). intro X. inv X; simplify. rename c into wl, d into rl.
+  destruct n.
+  { generalize (lastn_length 1 tr). rewrite EU. destruct tr; ss. }
+  exploit sim_trace_lastn; eauto. instantiate (1 := S n). intro SIMTR.
+  exploit sim_traces_ex; eauto. intro EX2.
+  inversion SIMTR; subst; simplify; [congr|].
+  repeat match goal with
+         | [H1: lastn ?a ?b = ?c, H2: ?d = lastn ?a ?b |- _] =>
+           rewrite H1 in H2; inv H2
+         end.
+  exploit sim_trace_sim_state_weak; eauto. intro STATE1.
+  rename H2 into WS, H3 into RS, H4 into WL, H5 into RL.
+
+  ii.
+  destruct (le_lt_dec (length (ALocal.labels (AExecUnit.local aeu1))) eid1); cycle 1.
+  { eapply L; eauto. }
+  assert (LABEL1: Execution.label_is ex (fun label : Label.t => Label.is_read label) (tid, eid1)).
+  { admit. }
+  inv LABEL1. destruct l0; ss.
+  destruct eu1 as [st1 lc1 mem1].
+  destruct eu2 as [st2 lc2 mem2].
+  destruct aeu1 as [ast1 alc1].
+  destruct aeu2 as [ast2 alc2].
+  inv ASTATE_STEP; inv EVENT; inv ALOCAL_STEP; inv EVENT; repeat (ss; subst).
+  all: try (clear - LABEL l; lia).
+  all: rewrite List.app_length in LABEL; ss.
+  all: assert (EID1: eid1 = length (ALocal.labels alc1)) by (clear - LABEL l; lia); subst.
+  all: exploit LABELS; eauto; ss.
+  all: try by clear; rewrite List.app_length; s; lia.
+  all: intro NTH; apply nth_error_snoc_inv_last in NTH; des; try lia.
+  all: inv NTH.
+  rewrite EU, AEU, COV, VEXT, <- WL, <- RL in SIMTR.
+  exploit sim_trace_sim_th; try exact SIMTR; eauto. intro L'.
+  exploit L'.(RPROP1); ss.
+  { apply nth_error_last. apply Nat.eqb_eq. ss. }
+  unfold ALocal.next_eid in *. condtac; cycle 1.
+  { apply Nat.eqb_neq in X. congr. }
+  exploit L'.(RPROP2); ss.
+  { rewrite X. eauto. }
+  rewrite X. i. des. inv x1. apply nth_error_snoc_inv_last in x4. inv x4.
+  clear x0 x3 x5 tid'0.
+  rewrite EX2.(XVEXT); s; cycle 1.
+  { rewrite List.app_length. s. clear. lia. }
+  rewrite X. 
+  inv STEP0. ss. subst. inv LOCAL0; inv EVENT.
+  admit. (* should be true from STEP0 *)
+
+  (* ii. inversion FR0. *)
+  (* - admit. (* read from non-initial value *) *)
+  (* - inv H. inv H1. inv H. inv H1. *)
+  (*   exploit LABELS; eauto. intro LABEL1. destruct l; ss. *)
+  (*   rewrite EU, AEU, COV, VEXT, <- WL, <- RL in SIMTR. *)
+  (*   exploit sim_trace_sim_th; try exact SIMTR; eauto. intro L'. *)
+  (*   exploit L'.(RPROP1); eauto. i. des. unguardH x1. des. *)
+  (*   + subst. *)
+  (*     inv EVENT; ss. *)
+  (*     * eapply FR; eauto. inv ALOCAL_STEP; ss. *)
+  (*     * des_ifs; cycle 1. *)
+  (*       { eapply FR; eauto. inv ALOCAL_STEP; ss. *)
+  (*         eapply nth_error_not_last; eauto. } *)
+  (*       { inv STEP0. ss. inv LOCAL0; ss. inv STEP0. inv EVENT. ss. *)
+  (*         rewrite fun_add_spec in H1. *)
+  (*         destruct (equiv_dec (ValA.val vloc) (ValA.val vloc)); try congr. *)
+  (*         admit. *)
+  (*       } *)
+  (*     * inv STEP0. ss. inv LOCAL0; ss; inv EVENT. *)
+  (*       { inv STEP0. ss. inv ALOCAL_STEP; ss. *)
+  (*         - destruct (Nat.eqb eid1 (ALocal.next_eid alc1)) eqn:HEID1. *)
+  (*           + rewrite nth_error_last in LABEL1; auto. inv LABEL1. *)
+  (*           + eapply FR; eauto. eapply nth_error_not_last; eauto. *)
+  (*         - inv EVENT. inv RES. ss. } *)
+  (*       { inv STEP0. ss. eapply FR; eauto. inv ALOCAL_STEP; ss. *)
+  (*         destruct (Nat.eqb eid1 (List.length (ALocal.labels alc1))) eqn:HEID1. *)
+  (*         - rewrite nth_error_last in LABEL1; eauto. inv LABEL1. *)
+  (*         - eapply nth_error_not_last; eauto. } *)
+  (*     * inv STEP0. ss. inv LOCAL0; ss; inv EVENT. *)
+  (*       { inv STEP0. ss. eapply FR; eauto. inv ALOCAL_STEP; ss. *)
+  (*         destruct (Nat.eqb eid1 (List.length (ALocal.labels alc1))) eqn:HEID1. *)
+  (*         - rewrite nth_error_last in LABEL1; eauto. inv LABEL1. *)
+  (*         - eapply nth_error_not_last; eauto. } *)
+  (*       { inv STEP0. ss. eapply FR; eauto. inv ALOCAL_STEP; ss. *)
+  (*         destruct (Nat.eqb eid1 (List.length (ALocal.labels alc1))) eqn:HEID1. *)
+  (*         - rewrite nth_error_last in LABEL1; eauto. inv LABEL1. *)
+  (*         - eapply nth_error_not_last; eauto. } *)
+  (*     * inv STEP0. ss. inv LOCAL0; ss; inv EVENT. *)
+  (*       inv LC0. ss. eapply FR; eauto. inv ALOCAL_STEP; ss. *)
+  (*       destruct (Nat.eqb eid1 (List.length (ALocal.labels alc1))) eqn:HEID1. *)
+  (*       { rewrite nth_error_last in LABEL1; eauto. inv LABEL1. } *)
+  (*       { eapply nth_error_not_last; eauto. } *)
+  (*   + exploit sim_traces_memory; eauto. i. des. *)
+  (*     generalize (SIM tid'). intro SIM'. inv SIM'; try congr. simplify. *)
+  (*     exploit sim_trace_last; try exact REL0. i. des. subst. *)
+  (*     exploit sim_trace_sim_th; try exact REL0; eauto. i. destruct x3. *)
+  (*     exploit WPROP0; eauto. i. des. *)
+  (*     * inv STEP. inv NOPROMISE. *)
+  (*       generalize (TR tid'). intro TR'. inv TR'; try congr. des. simplify. *)
+  (*       destruct b. exploit PROMISES0; eauto. i. *)
+  (*       ss. rewrite x4 in *. rewrite Promises.lookup_bot in x1. ss. *)
+  (*     * exfalso. apply H3. econs. rewrite RF. *)
+  (*       instantiate (1 := (tid', eid)). *)
+  (*       exploit sim_trace_last; try exact REL6. i. des. subst. *)
+  (*       econs; try refl; ss; eauto. *)
+  (*       admit. (* should prove that r includes r2 *) *)
+Admitted.
