src/axiomatic/PFtoA4OBR.v
@@ -1,0 +1,109 @@
+Require Import Relations.
+Require Import Permutation.
+Require Import NArith.
+Require Import PArith.
+Require Import ZArith.
+Require Import Lia.
+Require Import FMapPositive.
+Require Import FSetPositive.
+Require Import EquivDec.
+Require Import sflib.
+Require Import paco.
+Require Import HahnRelationsBasic.
+Require Import HahnSets.
+
+Require Import PromisingArch.lib.Basic.
+Require Import PromisingArch.lib.HahnRelationsMore.
+Require Import PromisingArch.lib.Order.
+Require Import PromisingArch.lib.Time.
+Require Import PromisingArch.lib.Lang.
+Require Import PromisingArch.promising.Promising.
+Require Import PromisingArch.promising.StateExecFacts.
+Require Import PromisingArch.axiomatic.Axiomatic.
+Require Import PromisingArch.axiomatic.CommonAxiomatic.
+Require Import PromisingArch.axiomatic.PFtoA1.
+Require Import PromisingArch.axiomatic.PFtoA2.
+Require Import PromisingArch.axiomatic.PFtoA3.
+
+Set Implicit Arguments.
+
+
+Lemma sim_traces_sim_th'_ob_read
+      p trs atrs ws rs covs vexts
+      m ex
+      (STEP: Machine.pf_exec p m)
+      (SIM: sim_traces p m.(Machine.mem) trs atrs ws rs covs vexts)
+      (PRE: Valid.pre_ex p ex)
+      (CO: ex.(Execution.co) = co_gen ws)
+      (RF: ex.(Execution.rf) = rf_gen ws rs)
+      (CO1: Valid.co1 ex)
+      (CO2: Valid.co2 ex)
+      (RF1: Valid.rf1 ex)
+      (RF2: Valid.rf2 ex)
+      (RF_WF: Valid.rf_wf ex)
+      (TR: IdMap.Forall2
+             (fun _ tr sl => exists l, tr = (ExecUnit.mk sl.(fst) sl.(snd) m.(Machine.mem)) :: l)
+             trs m.(Machine.tpool))
+      (ATR: IdMap.Forall2
+              (fun _ atr aeu => exists l, atr = aeu :: l)
+              atrs (Valid.aeus PRE)):
+  forall tid tr atr covl vextl
+    n eu1 eu2 tr' aeu1 aeu2 atr' cov1 cov2 covl' vext1 vext2 vextl'
+    (FIND_TR: IdMap.find tid trs = Some tr)
+    (FIND_ATR: IdMap.find tid atrs = Some atr)
+    (FIND_COVL: IdMap.find tid covs = Some covl)
+    (FIND_VEXTL: IdMap.find tid vexts = Some vextl)
+    (EU: lastn (S n) tr = eu2 :: eu1 :: tr')
+    (AEU: lastn (S n) atr = aeu2 :: aeu1 :: atr')
+    (COV: lastn (S n) covl = cov2 :: cov1 :: covl')
+    (VEXT: lastn (S n) vextl = vext2 :: vext1 :: vextl')
+    (SIM_TH': sim_th' tid ex (v_gen vexts) eu1 aeu1),
+    sim_ob_read tid ex (v_gen vexts) eu2 aeu2.
+Proof.
+  i. rename SIM_TH' into L.
+  generalize (SIM tid). intro X. inv X; simplify. rename c into wl, d into rl.
+  destruct n.
+  { generalize (lastn_length 1 tr). rewrite EU. destruct tr; ss. }
+  exploit sim_trace_lastn; eauto. instantiate (1 := S n). intro SIMTR.
+  exploit sim_traces_ex; eauto. intro EX2.
+  inversion SIMTR; subst; simplify; [congr|].
+  repeat match goal with
+         | [H1: lastn ?a ?b = ?c, H2: ?d = lastn ?a ?b |- _] =>
+           rewrite H1 in H2; inv H2
+         end.
+  exploit sim_trace_sim_state_weak; eauto. intro STATE1.
+  rename H2 into WS, H3 into RS, H4 into WL, H5 into RL.
+
+  ii.
+  destruct (le_lt_dec (length (ALocal.labels (AExecUnit.local aeu1))) eid2); cycle 1.
+  { eapply L; eauto. }
+  inv EID2. destruct l0; ss.
+  destruct eu1 as [st1 lc1 mem1].
+  destruct eu2 as [st2 lc2 mem2].
+  destruct aeu1 as [ast1 alc1].
+  destruct aeu2 as [ast2 alc2].
+  inv ASTATE_STEP; inv EVENT; inv ALOCAL_STEP; inv EVENT; repeat (ss; subst).
+  all: try (clear - LABEL l; lia).
+  all: rewrite List.app_length in LABEL; ss.
+  all: assert (EID2: eid2 = length (ALocal.labels alc1)) by (clear - LABEL l; lia); subst.
+  all: exploit LABELS; eauto; ss.
+  all: try by clear; rewrite List.app_length; s; lia.
+  all: intro NTH; apply nth_error_snoc_inv_last in NTH; des; try lia.
+  all: inv NTH.
+  rewrite EU, AEU, COV, VEXT, <- WL, <- RL in SIMTR.
+  exploit sim_trace_sim_th; try exact SIMTR; eauto. intro L'.
+  exploit L'.(RPROP1); ss.
+  { apply nth_error_last. apply Nat.eqb_eq. ss. }
+  unfold ALocal.next_eid in *. condtac; cycle 1.
+  { apply Nat.eqb_neq in X. congr. }
+  i. des. inv x0.
+  exploit L'.(RPROP2); eauto.
+  { rewrite X. eauto. }
+  s. rewrite X. i. des.
+  apply nth_error_snoc_inv_last in x3. inv x3.
+  clear x4 H3 tid'0 x2 x0.
+  rewrite EX2.(XVEXT); s; cycle 1.
+  { rewrite List.app_length. s. clear. lia. }
+  rewrite X. 
+  move AOB at bottom. admit.
+Admitted.
