src/axiomatic/PFtoA4SL.v
@@ -1,0 +1,432 @@
+Require Import Relations.
+Require Import Permutation.
+Require Import NArith.
+Require Import PArith.
+Require Import ZArith.
+Require Import Lia.
+Require Import FMapPositive.
+Require Import FSetPositive.
+Require Import EquivDec.
+Require Import sflib.
+Require Import paco.
+Require Import HahnRelationsBasic.
+Require Import HahnSets.
+
+Require Import PromisingArch.lib.Basic.
+Require Import PromisingArch.lib.HahnRelationsMore.
+Require Import PromisingArch.lib.Order.
+Require Import PromisingArch.lib.Time.
+Require Import PromisingArch.lib.Lang.
+Require Import PromisingArch.promising.Promising.
+Require Import PromisingArch.promising.StateExecFacts.
+Require Import PromisingArch.axiomatic.Axiomatic.
+Require Import PromisingArch.axiomatic.CommonAxiomatic.
+Require Import PromisingArch.axiomatic.PFtoA1.
+Require Import PromisingArch.axiomatic.PFtoA2.
+Require Import PromisingArch.axiomatic.PFtoA3.
+
+Set Implicit Arguments.
+
+
+Lemma sim_traces_sim_th'_sl
+      p trs atrs ws rs covs vexts
+      m ex
+      (STEP: Machine.pf_exec p m)
+      (SIM: sim_traces p m.(Machine.mem) trs atrs ws rs covs vexts)
+      (PRE: Valid.pre_ex p ex)
+      (CO: ex.(Execution.co) = co_gen ws)
+      (RF: ex.(Execution.rf) = rf_gen ws rs)
+      (CO1: Valid.co1 ex)
+      (CO2: Valid.co2 ex)
+      (RF1: Valid.rf1 ex)
+      (RF2: Valid.rf2 ex)
+      (RF_WF: Valid.rf_wf ex)
+      (TR: IdMap.Forall2
+             (fun _ tr sl => exists l, tr = (ExecUnit.mk sl.(fst) sl.(snd) m.(Machine.mem)) :: l)
+             trs m.(Machine.tpool))
+      (ATR: IdMap.Forall2
+              (fun _ atr aeu => exists l, atr = aeu :: l)
+              atrs (Valid.aeus PRE)):
+  forall tid tr atr covl vextl
+    n eu1 eu2 tr' aeu1 aeu2 atr' cov1 cov2 covl' vext1 vext2 vextl'
+    (FIND_TR: IdMap.find tid trs = Some tr)
+    (FIND_ATR: IdMap.find tid atrs = Some atr)
+    (FIND_COVL: IdMap.find tid covs = Some covl)
+    (FIND_VEXTL: IdMap.find tid vexts = Some vextl)
+    (EU: lastn (S n) tr = eu2 :: eu1 :: tr')
+    (AEU: lastn (S n) atr = aeu2 :: aeu1 :: atr')
+    (COV: lastn (S n) covl = cov2 :: cov1 :: covl')
+    (VEXT: lastn (S n) vextl = vext2 :: vext1 :: vextl')
+    (SIM_TH': sim_th' tid ex (v_gen vexts) eu1 aeu1),
+    sim_state tid (v_gen vexts) eu2.(ExecUnit.state) aeu2.(AExecUnit.state) /\
+    sim_local tid ex (v_gen vexts) eu2.(ExecUnit.local) aeu2.(AExecUnit.local).
+Proof.
+  i. rename SIM_TH' into L.
+  generalize (SIM tid). intro X. inv X; simplify. rename c into wl, d into rl.
+  destruct n.
+  { generalize (lastn_length 1 tr). rewrite EU. destruct tr; ss. }
+  exploit sim_trace_lastn; eauto. instantiate (1 := S n). intro SIMTR.
+  exploit sim_traces_ex; eauto. intro EX2.
+  inversion SIMTR; subst; simplify; [congr|].
+  repeat match goal with
+         | [H1: lastn ?a ?b = ?c, H2: ?d = lastn ?a ?b |- _] =>
+           rewrite H1 in H2; inv H2
+         end.
+  exploit sim_trace_sim_state_weak; eauto. intro STATE1.
+  rename H2 into WS, H3 into RS, H4 into WL, H5 into RL.
+
+  destruct eu1 as [[stmts1 rmap1] lc1 mem1].
+  destruct eu2 as [[stmts2 rmap2] lc2 mem2].
+  destruct aeu1 as [[astmts1 armap1] alc1].
+  destruct aeu2 as [[astmts2 armap2] alc2].
+  ss. inv STEP0. ss. subst.
+  inv STATE. inv STATE1. ss. subst.
+  inv STATE0; inv LOCAL0; ss; inv EVENT0; inv EVENT; ss.
+  - (* skip *)
+    inv ASTATE_STEP; inv ALOCAL_STEP; ss; inv EVENT; ss. splits.
+    + econs; ss. apply L.
+    + econs; ss; try by apply L.
+  - (* assign *)
+    inv ASTATE_STEP; inv ALOCAL_STEP; ss; inv EVENT; ss. splits.
+    + econs; ss. apply sim_rmap_add; try by apply L.
+      apply sim_rmap_expr. apply L.
+    + econs; ss; try by apply L.
+  - (* read *)
+    admit.
+  - (* write *)
+    admit.
+  (* econs; ss. *)
+  (* { econs; ss. apply sim_rmap_add; ss. inv STEP. econs; ss. *)
+  (*   ii. des. subst. destruct (equiv_dec arch riscv); ss. destruct eid. ss. subst. *)
+  (*   unfold ALocal.next_eid in *. *)
+  (*   rewrite VEXT1; cycle 1. *)
+  (*   { rewrite List.app_length. s. clear. lia. } *)
+  (*   condtac; cycle 1. *)
+  (*   { apply Nat.eqb_neq in X. ss. } *)
+  (*   rewrite fun_add_spec. condtac; ss. *)
+  (*   inv WRITABLE. apply Nat.lt_le_incl. ss. *)
+  (* } *)
+  - (* write failure *)
+    inv STEP0. inv RES. inv ASTATE_STEP; inv ALOCAL_STEP; ss; inv EVENT; ss. splits.
+    + econs; ss. apply sim_rmap_add; try by apply L. econs; ss. ii. des. ss.
+    + econs; ss; try by apply L.
+  - (* isb *)
+    inv STEP0. inv ASTATE_STEP; inv ALOCAL_STEP; ss; inv EVENT; ss. splits.
+    econs; ss.
+    { econs; ss. apply L. }
+    destruct L.(LC). ss. econs; ss.
+    + rewrite List.app_length, Nat.add_1_r.
+      i. rewrite sim_local_coh_step. rewrite inverse_step.
+      rewrite inverse_union. ii. des; [apply COH|]; eauto.
+      inv EID. inv REL. inv H. inv H0. inv H2.
+      apply Label.is_writing_inv in LABEL. des. subst. inv H1.
+      * exploit EX2.(LABELS); eauto; ss; cycle 1.
+        { rewrite List.nth_error_app2, Nat.sub_diag; ss. }
+        { rewrite List.app_length. s. lia. }
+      * inv H. exploit RF2; eauto. i. des.
+        exploit EX2.(LABELS); eauto; ss; cycle 1.
+        { rewrite List.nth_error_app2, Nat.sub_diag; ss. }
+        { rewrite List.app_length. s. lia. }
+    + rewrite List.app_length, Nat.add_1_r.
+      i. rewrite sim_local_vrp_step. rewrite inverse_step.
+      rewrite ? inverse_union. ii. des.
+      * exploit VRP; eauto. i. rewrite <- join_l. ss.
+      * inv EID. inv REL. inv H. inv H1. inv H. inv H2. inv H3.
+        exploit EX2.(LABELS); eauto; ss.
+        { rewrite List.app_length. s. lia. }
+        { rewrite List.nth_error_app2, Nat.sub_diag; ss. i. inv x1. inv LABEL. }
+      * inv EID. inv REL. inv H. inv H1. inv H. inv H2. inv H3.
+        exploit EX2.(LABELS); eauto; ss.
+        { rewrite List.app_length. s. lia. }
+        { rewrite List.nth_error_app2, Nat.sub_diag; ss. i. inv x1. inv LABEL. }
+      * inv EID. inv REL. inv H. inv H1.
+        rewrite <- join_r. apply L. econs; eauto.
+      * inv EID. inv REL. inv H0. destruct l; ss.
+        exploit EX2.(LABELS); eauto; ss; cycle 1.
+        { rewrite List.nth_error_app2, Nat.sub_diag; ss. }
+        { rewrite List.app_length. s. lia. }
+    + rewrite List.app_length, Nat.add_1_r.
+      i. rewrite sim_local_vwp_step. rewrite inverse_step.
+      rewrite ? inverse_union. ii. des.
+      * exploit VWP; eauto.
+      * inv EID. inv REL. inv H. inv H1. inv H. inv H2. inv H3.
+        exploit EX2.(LABELS); eauto; ss.
+        { rewrite List.app_length. s. lia. }
+        { rewrite List.nth_error_app2, Nat.sub_diag; ss. i. inv x1. inv LABEL. }
+      * inv EID. inv REL. inv H. inv H1. inv H. inv H2. inv H3.
+        exploit EX2.(LABELS); eauto; ss.
+        { rewrite List.app_length. s. lia. }
+        { rewrite List.nth_error_app2, Nat.sub_diag; ss. i. inv x1. inv LABEL. }
+      * inv EID. inv REL. inv H0. destruct l; ss.
+        exploit EX2.(LABELS); eauto; ss; cycle 1.
+        { rewrite List.nth_error_app2, Nat.sub_diag; ss. }
+        { rewrite List.app_length. s. lia. }
+    + rewrite List.app_length, Nat.add_1_r.
+      i. rewrite sim_local_vrm_step. rewrite inverse_step.
+      rewrite ? inverse_union. ii. des.
+      * exploit VRM; eauto.
+      * inv EID. inv REL. inv H0. destruct l; ss.
+        exploit EX2.(LABELS); eauto; ss; cycle 1.
+        { rewrite List.nth_error_app2, Nat.sub_diag; ss. }
+        { rewrite List.app_length. s. lia. }
+    + rewrite List.app_length, Nat.add_1_r.
+      i. rewrite sim_local_vwm_step. rewrite inverse_step.
+      rewrite ? inverse_union. ii. des.
+      * exploit VWM; eauto.
+      * inv EID. inv REL. inv H0. destruct l; ss.
+        exploit EX2.(LABELS); eauto; ss; cycle 1.
+        { rewrite List.nth_error_app2, Nat.sub_diag; ss. }
+        { rewrite List.app_length. s. lia. }
+    + (* vcap *)
+      rewrite List.app_length, Nat.add_1_r.
+      i. rewrite sim_local_vcap_step. rewrite inverse_step.
+      rewrite inverse_union. ii. des.
+      * exploit VCAP; eauto.
+      * admit. (* ctrl/addr doesn't flow into barrier *)
+
+    (* * (* TODO: move *) *)
+    (*   Lemma addr_po_step ex: *)
+    (*     (ex.(Execution.addr) ⨾ Execution.po) = *)
+    (*     ((ex.(Execution.addr) ⨾ Execution.po) ∪ ex.(Execution.addr)) ⨾ *)
+    (*                                                                  Execution.po_adj. *)
+    (*   Proof. *)
+    (*     rewrite ? (union_seq' Execution.po_adj), ? seq_assoc, ? union_assoc. *)
+    (*     rewrite Execution.po_po_adj at 1. *)
+    (*     rewrite (clos_refl_union Execution.po), union_seq, eq_seq. *)
+    (*     rewrite ? (seq_union' (Execution.po ⨾ Execution.po_adj) Execution.po_adj), ? seq_assoc, ? union_assoc. *)
+    (*     refl. *)
+    (*   Qed. *)
+        
+    (*   rewrite addr_po_step in H. *)
+        
+    (*   (*TODO: move *) *)
+    (*   Lemma step r eid tid n: *)
+    (*     (r ⨾ Execution.po_adj) eid (tid, S n) = r eid (tid, n). *)
+    (*   Proof. *)
+    (*     propext. econs; i. *)
+    (*     - inv H. des. inv H1. destruct x. ss. inv N. auto. *)
+    (*     - econs. split; eauto. *)
+    (*   Qed. *)
+
+    (*   rewrite step in H. *)
+    (*   inv H. *)
+    (*   { eapply VCAP; eauto. econs; eauto. econs 2; eauto. } *)
+    (*   { (* TODO: move *) *)
+    (*     Lemma addr_eid *)
+    (*           p ex (PRE: Valid.pre_ex p ex) *)
+    (*           eid tid eid2 *)
+    (*           (ADDR: ex.(Execution.addr) eid (tid, eid2)): *)
+    (*       exists eid1, eid = (tid, eid1). *)
+    (*     Proof. *)
+    (*     Admitted. *)
+
+    (*     exploit addr_eid; eauto. i. des. subst. *)
+    (*     exploit ADDR; eauto; ss. *)
+    (*     { rewrite List.app_length. ss. clear. lia. } *)
+    (*     i. *)
+
+    (*     (* TODO: move *) *)
+    (*     Lemma addr_inv *)
+    (*           p mem tid tr aeu atr wl rl covl vextl *)
+    (*           eid1 eid2 *)
+    (*           (SIM: sim_trace p mem tid tr (aeu::atr) wl rl covl vextl) *)
+    (*           (EID2: eid2 >= List.length aeu.(AExecUnit.local).(ALocal.labels)) *)
+    (*           (ADDR: aeu.(AExecUnit.local).(ALocal.addr) eid1 eid2): *)
+    (*       False. *)
+    (*     Proof. *)
+    (*     Admitted. *)
+
+    (*     exploit addr_inv; eauto. ss. *)
+    (*   } *)
+    + rewrite List.app_length, Nat.add_1_r.
+      i. rewrite sim_local_vrel_step. rewrite inverse_step.
+      rewrite ? inverse_union. ii. des.
+      * exploit VREL; eauto.
+      * inv EID. inv REL. inv H0. destruct l; ss.
+        exploit EX2.(LABELS); eauto; ss.
+        { rewrite List.app_length. s. lia. }
+        { rewrite List.nth_error_app2, Nat.sub_diag; ss. }
+    + admit. (* fwdbank *)
+    + admit. (* promise *)
+  - (* dmb *)
+    inv STEP0. inv ASTATE_STEP; inv ALOCAL_STEP; ss; inv EVENT; ss. splits.
+    econs; ss.
+    { econs; ss. apply L. }
+    destruct L.(LC). ss. econs; ss.
+    + rewrite List.app_length, Nat.add_1_r.
+      i. rewrite sim_local_coh_step. rewrite inverse_step.
+      rewrite inverse_union. ii. des; [apply COH|]; eauto.
+      inv EID. inv REL. inv H. inv H0. inv H2.
+      apply Label.is_writing_inv in LABEL. des. subst. inv H1.
+      * exploit EX2.(LABELS); eauto; ss; cycle 1.
+        { rewrite List.nth_error_app2, Nat.sub_diag; ss. }
+        { rewrite List.app_length. s. lia. }
+      * inv H. exploit RF2; eauto. i. des.
+        exploit EX2.(LABELS); eauto; ss; cycle 1.
+        { rewrite List.nth_error_app2, Nat.sub_diag; ss. }
+        { rewrite List.app_length. s. lia. }
+    + rewrite List.app_length, Nat.add_1_r.
+      i. rewrite sim_local_vrp_step. rewrite inverse_step.
+      rewrite ? inverse_union. ii. des.
+      * exploit VRP; eauto. i. rewrite <- join_l. ss.
+      * inv EID. inv REL. inv H. inv H1. inv H. inv H2. inv H3.
+        exploit EX2.(LABELS); eauto; ss.
+        { rewrite List.app_length. s. lia. }
+        rewrite List.nth_error_app2, Nat.sub_diag; ss. i. simplify.
+        destruct rr; ss.
+        rewrite <- join_r, <- join_l. apply L. econs; eauto. econs; eauto.
+      * inv EID. inv REL. inv H. inv H1. inv H. inv H2. inv H3.
+        exploit EX2.(LABELS); eauto; ss.
+        { rewrite List.app_length. s. lia. }
+        rewrite List.nth_error_app2, Nat.sub_diag; ss. i. simplify.
+        destruct wr; ss.
+        rewrite <- join_r, <- join_r, <- join_l. apply L. econs; eauto. econs; eauto.
+      * inv EID. inv REL. inv H. inv H1. inv H2.
+        exploit EX2.(LABELS); eauto; ss.
+        { rewrite List.app_length. s. lia. }
+        { rewrite List.nth_error_app2, Nat.sub_diag; ss. }
+      * inv EID. inv REL. inv H0. destruct l; ss.
+        exploit EX2.(LABELS); eauto; ss.
+        { rewrite List.app_length. s. lia. }
+        { rewrite List.nth_error_app2, Nat.sub_diag; ss. }
+    + rewrite List.app_length, Nat.add_1_r.
+      i. rewrite sim_local_vwp_step. rewrite inverse_step.
+      rewrite ? inverse_union. ii. des.
+      * exploit VWP; eauto. i. rewrite <- join_l. ss.
+      * inv EID. inv REL. inv H. inv H1. inv H. inv H2. inv H3.
+        exploit EX2.(LABELS); eauto; ss.
+        { rewrite List.app_length. s. lia. }
+        rewrite List.nth_error_app2, Nat.sub_diag; ss. i. simplify.
+        destruct rw; ss.
+        rewrite <- join_r, <- join_l. apply L. econs; eauto. econs; eauto.
+      * inv EID. inv REL. inv H. inv H1. inv H. inv H2. inv H3.
+        exploit EX2.(LABELS); eauto; ss.
+        { rewrite List.app_length. s. lia. }
+        rewrite List.nth_error_app2, Nat.sub_diag; ss. i. simplify.
+        destruct ww; ss.
+        rewrite <- join_r, <- join_r, <- join_l. apply L. econs; eauto. econs; eauto.
+      * inv EID. inv REL. inv H0. destruct l; ss.
+        exploit EX2.(LABELS); eauto; ss.
+        { rewrite List.app_length. s. lia. }
+        { rewrite List.nth_error_app2, Nat.sub_diag; ss. }
+    + rewrite List.app_length, Nat.add_1_r.
+      i. rewrite sim_local_vrm_step. rewrite inverse_step.
+      rewrite ? inverse_union. ii. des.
+      * exploit VRM; eauto.
+      * inv EID. inv REL. inv H0. destruct l; ss.
+        exploit EX2.(LABELS); eauto; ss; cycle 1.
+        { rewrite List.nth_error_app2, Nat.sub_diag; ss. }
+        { rewrite List.app_length. s. lia. }
+    + rewrite List.app_length, Nat.add_1_r.
+      i. rewrite sim_local_vwm_step. rewrite inverse_step.
+      rewrite ? inverse_union. ii. des.
+      * exploit VWM; eauto.
+      * inv EID. inv REL. inv H0. destruct l; ss.
+        exploit EX2.(LABELS); eauto; ss; cycle 1.
+        { rewrite List.nth_error_app2, Nat.sub_diag; ss. }
+        { rewrite List.app_length. s. lia. }
+    + rewrite List.app_length, Nat.add_1_r.
+      i. rewrite sim_local_vcap_step. rewrite inverse_step.
+      rewrite inverse_union. ii. des.
+      * exploit VCAP; eauto.
+      * admit. (* ctrl/addr doesn't flow into barrier *)
+    + rewrite List.app_length, Nat.add_1_r.
+      i. rewrite sim_local_vrel_step. rewrite inverse_step.
+      rewrite ? inverse_union. ii. des.
+      * exploit VREL; eauto.
+      * inv EID. inv REL. inv H0. destruct l; ss.
+        exploit EX2.(LABELS); eauto; ss.
+        { rewrite List.app_length. s. lia. }
+        { rewrite List.nth_error_app2, Nat.sub_diag; ss. }
+    + admit. (* fwdbank *)
+    + admit. (* promise *)
+  - (* if *)
+    inv LC0. inv ASTATE_STEP; inv ALOCAL_STEP; ss; inv EVENT; ss. splits.
+    econs; ss.
+    { econs; ss. apply L. }
+    destruct L.(LC). ss. econs; ss.
+    + rewrite List.app_length, Nat.add_1_r.
+      i. rewrite sim_local_coh_step. rewrite inverse_step.
+      rewrite inverse_union. ii. des; [apply COH|]; eauto.
+      inv EID. inv REL. inv H. inv H0. inv H2.
+      apply Label.is_writing_inv in LABEL. des. subst. inv H1.
+      * exploit EX2.(LABELS); eauto; ss; cycle 1.
+        { rewrite List.nth_error_app2, Nat.sub_diag; ss. }
+        { rewrite List.app_length. s. lia. }
+      * inv H. exploit RF2; eauto. i. des.
+        exploit EX2.(LABELS); eauto; ss; cycle 1.
+        { rewrite List.nth_error_app2, Nat.sub_diag; ss. }
+        { rewrite List.app_length. s. lia. }
+    + rewrite List.app_length, Nat.add_1_r.
+      i. rewrite sim_local_vrp_step. rewrite inverse_step.
+      rewrite ? inverse_union. ii. des.
+      * exploit VRP; eauto.
+      * inv EID. inv REL. inv H. inv H1. inv H. inv H2. inv H3.
+        exploit EX2.(LABELS); eauto; ss.
+        { rewrite List.app_length. s. lia. }
+        rewrite List.nth_error_app2, Nat.sub_diag; ss. i. simplify. ss.
+      * inv EID. inv REL. inv H. inv H1. inv H. inv H2. inv H3.
+        exploit EX2.(LABELS); eauto; ss.
+        { rewrite List.app_length. s. lia. }
+        rewrite List.nth_error_app2, Nat.sub_diag; ss. i. simplify. ss.
+      * inv EID. inv REL. inv H. inv H1. inv H2.
+        exploit EX2.(LABELS); eauto; ss.
+        { rewrite List.app_length. s. lia. }
+        { rewrite List.nth_error_app2, Nat.sub_diag; ss. }
+      * inv EID. inv REL. inv H0. destruct l; ss.
+        exploit EX2.(LABELS); eauto; ss.
+        { rewrite List.app_length. s. lia. }
+        { rewrite List.nth_error_app2, Nat.sub_diag; ss. }
+    + rewrite List.app_length, Nat.add_1_r.
+      i. rewrite sim_local_vwp_step. rewrite inverse_step.
+      rewrite ? inverse_union. ii. des.
+      * exploit VWP; eauto.
+      * inv EID. inv REL. inv H. inv H1. inv H. inv H2. inv H3.
+        exploit EX2.(LABELS); eauto; ss.
+        { rewrite List.app_length. s. lia. }
+        rewrite List.nth_error_app2, Nat.sub_diag; ss. i. simplify. ss.
+      * inv EID. inv REL. inv H. inv H1. inv H. inv H2. inv H3.
+        exploit EX2.(LABELS); eauto; ss.
+        { rewrite List.app_length. s. lia. }
+        rewrite List.nth_error_app2, Nat.sub_diag; ss. i. simplify. ss.
+      * inv EID. inv REL. inv H0. destruct l; ss.
+        exploit EX2.(LABELS); eauto; ss.
+        { rewrite List.app_length. s. lia. }
+        { rewrite List.nth_error_app2, Nat.sub_diag; ss. }
+    + rewrite List.app_length, Nat.add_1_r.
+      i. rewrite sim_local_vrm_step. rewrite inverse_step.
+      rewrite ? inverse_union. ii. des.
+      * exploit VRM; eauto.
+      * inv EID. inv REL. inv H0. destruct l; ss.
+        exploit EX2.(LABELS); eauto; ss; cycle 1.
+        { rewrite List.nth_error_app2, Nat.sub_diag; ss. }
+        { rewrite List.app_length. s. lia. }
+    + rewrite List.app_length, Nat.add_1_r.
+      i. rewrite sim_local_vwm_step. rewrite inverse_step.
+      rewrite ? inverse_union. ii. des.
+      * exploit VWM; eauto.
+      * inv EID. inv REL. inv H0. destruct l; ss.
+        exploit EX2.(LABELS); eauto; ss; cycle 1.
+        { rewrite List.nth_error_app2, Nat.sub_diag; ss. }
+        { rewrite List.app_length. s. lia. }
+    + rewrite List.app_length, Nat.add_1_r.
+      i. rewrite sim_local_vcap_step. rewrite inverse_step.
+      rewrite inverse_union. ii. des.
+      * rewrite <- join_l. exploit VCAP; eauto.
+      * rewrite <- join_r.
+        admit. (* use EX2.(CTRL) .. *)
+    + rewrite List.app_length, Nat.add_1_r.
+      i. rewrite sim_local_vrel_step. rewrite inverse_step.
+      rewrite ? inverse_union. ii. des.
+      * exploit VREL; eauto.
+      * inv EID. inv REL. inv H0. destruct l; ss.
+        exploit EX2.(LABELS); eauto; ss.
+        { rewrite List.app_length. s. lia. }
+        { rewrite List.nth_error_app2, Nat.sub_diag; ss. }
+    + admit. (* fwdbank *)
+    + admit. (* promise *)
+  - (* dowhile *)
+    inv ASTATE_STEP; inv ALOCAL_STEP; ss; inv EVENT; ss. splits.
+    + econs; ss; try by apply L.
+    + econs; ss; try by apply L.
+Admitted.
